wip

fairness/examples/ticketlock/client_adequacy.v
@@ -1,5 +1,7 @@
-From trillium.fairness Require Import fairness fuel fairness_finiteness lm_fair comp_utils.
-From trillium.fairness.examples.ticketlock Require Import ticketlock_model_lm client_model ticketlock_model fair_lock_lm lm_restr client_trace_termination. 
+From trillium.fairness.heap_lang Require Import notation simulation_adequacy_lm heap_lang_defs em_lm_heap_lang.
+From trillium.fairness Require Import fairness fuel fairness_finiteness lm_fair comp_utils fair_termination lm_fairness_preservation lm_fairness_preservation_wip lm_fair_traces.
+From trillium.fairness.ext_models Require Import ext_models.
+From trillium.fairness.examples.ticketlock Require Import ticketlock_model_lm client_model ticketlock_model fair_lock lm_restr client_trace_termination fair_lock_lm. 
 
 Section Adequacy.
   Let M := tl_fair_model.
@@ -54,7 +56,96 @@ Section Adequacy.
       cl_pre_inG :> clientPreGS Σ;
     }.
 
+    Definition clientPreΣ : gFunctors :=
+      #[].
+    
+    Global Instance subG_clientPreΣ {Σ}:
+      subG clientPreΣ Σ → clientPreGS Σ.
+    Qed. 
+
+    Definition client: val.
+    Admitted. 
+
   End tmp.
+
+  (* TODO: adapt proof in comp/lib_ext.v *)
+  Lemma lib_keeps_asg: ∀ (δ1 : fmstate LM_Fair) (ι : env_role) (δ2 : fmstate LM_Fair) (ρ: fmrole tl_fair_model) (τ: G) (f : nat),
+     @ext_trans _ (FL_EM tl_FLE) δ1 (Some (inr ι)) δ2
+     → ls_mapping δ1 !! ρ = Some τ
+       → ls_fuel δ1 !! ρ = Some f
+         → ls_mapping δ2 !! ρ = Some τ ∧ ls_fuel δ2 !! ρ = Some f.
+  Proof.
+  Admitted. 
+
+  Lemma client_LM_inner_exposed (auxtr: lmftrace (LM := client_model)):
+    inner_obls_exposed (option_fmap _ _ inl) (λ c δ_lib, c.1 = δ_lib) auxtr (LMo := client_model) (AMi := ELM_ALM lib_keeps_asg).
+    (*   inner_obls_exposed ((option_fmap _ _ inl) ext_role (ext_role + cl_id)%type inl) *)
+    (* (λ (st : client_model_impl) (tl_st : lm_ls TlLM), st.1 = tl_st) auxtr.  *)
+
+  Proof.
+    red. simpl. intros n δ gl NTH (?&?&?&MAP).
+    eexists. split; [reflexivity| ].
+    rewrite (ls_same_doms δ) mapped_roles_dom_fuels.
+    apply (ls_inv δ). rewrite H. eauto.
+  Qed.
+
+(* TODO: move, generalize *)
+Theorem simulation_adequacy_terminate_client (Σ: gFunctors)
+        {hPre: @heapGpreS Σ (fair_model_model (@LM_Fair _ _ _ _ _ _ client_LF)) (@LM_EM_HL _ _ client_model client_LF)} (s: stuckness)
+        e1 (s1: fmstate client_model_impl) FR
+        (LSI0: initial_ls_LSI s1 0 (M := client_model_impl) (LM := client_model) (LSI := client_LSI))
+        (INIT: is_init_cl_state s1)
+        (extr : heap_lang_extrace)
+        (Hexfirst : (trfirst extr).1 = [e1])
+  :
+  rel_finitary (sim_rel client_model (LF := client_LF)) →
+  wp_premise (λ _ _, True) (trfirst extr).2 e1 s1 s FR LSI0 ->
+  extrace_fairly_terminating extr.
+Proof.
+  intros Hfb Hwp Hvex Hfair.
+
+  destruct (simulation_adequacy_model_trace
+              Σ _ e1 s1 FR LSI0 extr Hvex Hexfirst Hfb Hwp) as (auxtr&mtr&Hmatch&Hupto&A0).
+
+  (* TODO: clarify which types of fairness we need in this proof *)
+  assert (forall ρ, fair_aux_SoU (LM_ALM client_model) ρ auxtr (LM := client_model)) as FAIR_SOU.
+  { apply group_fairness_implies_step_or_unassign; eauto.
+    { eapply traces_match_valid2; eauto. }
+    eapply fairness_preserved; eauto.
+    { apply _. }
+    { intros. apply match_locale_enabled_states_livetids. }
+    intros.
+    destruct ζ.
+    { apply Hfair. }
+    simpl. red. simpl in *. by intros ?(?&?&?)%pred_at_trace_lookup. }
+
+  pose proof (ex_fairness_preserved _ _ Hmatch Hfair) as Hfairaux'.
+  pose proof (proj1 (LM_ALM_afair_by_next _ auxtr) Hfairaux') as Hfairaux.  
+  
+  have Hfairm := lm_fair_traces.upto_stutter_fairness auxtr mtr Hupto Hfairaux.
+  pose proof (traces_match_valid2 _ _ _ _ _ _ Hmatch) as Hvalaux. 
+  have Hmtrvalid := lm_fair_traces.upto_preserves_validity auxtr mtr Hupto Hvalaux.
+
+  assert (mtrace_fairly_terminating mtr) as FAIR_TERM. 
+  { eapply client_model_fair_term.
+    2: { apply upto_stutter_trfirst in Hupto.
+         rewrite Hupto A0. simpl. done. } 
+    red. eexists. split; [| split]; eauto.
+    by apply client_LM_inner_exposed. }
+  assert (terminating_trace mtr) as Hterm.
+  { eapply FAIR_TERM; eauto. }
+    
+  eapply traces_match_preserves_termination =>//.
+  eapply lm_fair_traces.upto_stutter_finiteness =>//.
+Qed.
+
+  Definition δ0: fmstate TlLM_FM.
+  Admitted. 
+
+  Definition st0: fmstate client_model_impl := (δ0, fs_U).
+
+  Lemma st0_lsi: initial_ls_LSI st0 0 (LM := client_model).
+  Proof. Admitted. 
 
   Theorem client_terminates
     (extr : heap_lang_extrace)
@@ -62,14 +153,10 @@ Section Adequacy.
     (Hexfirst : (trfirst extr).1 = [client #()]):
     (∀ tid, fair_ex tid extr) -> terminating_trace extr.
   Proof.
-    set (Σ := gFunctors.app (heapΣ (@LM_EM_HL _ _ client_model LF')) clientPreΣ).
-    assert (heapGpreS Σ (@LM_EM_HL _ _ client_model LF')) as HPreG.
+    set (Σ := gFunctors.app (heapΣ (@LM_EM_HL _ _ client_model client_LF)) clientPreΣ).
+    assert (heapGpreS Σ (@LM_EM_HL _ _ client_model client_LF)) as HPreG.
     { apply _. }
-    set (st0 := (δ_lib0, 3): fmstate client_model_impl).
-    assert (initial_ls_LSI st0 0 (LM := client_model)) as LSI0.
-    { subst st0. red. red.
-      intros gi [ρ MAP]. simpl in MAP.
-      by rewrite δ_lib0_map in MAP. }
+    
     eapply (simulation_adequacy_terminate_client Σ NotStuck _ (st0: fmstate client_model_impl) _ LSI0); try done.
     - eapply valid_state_evolution_finitary_fairness_simple.
       apply client_model_finitary.
@@ -99,6 +186,3 @@ Section Adequacy.
   Qed.
 
 End Adequacy.
-
-
-
